StackMachine.v
@@ -1,0 +1,119 @@
+Require Import List.
+Import ListNotations.
+Require Import Omega.
+
+Require Export BigZ.
+Require Export Id.
+Require Export State.
+Require Export Expr.
+
+(* Sublist *)
+Fixpoint suffix (A : Type) (p : list A) (n : nat) :=
+  match n with
+  | 0   => p
+  | S k => match p with [] => [] | h :: tl => h :: suffix A tl k end
+  end.
+
+(* Stack machine instructions *)
+Inductive insn : Type :=
+| R  : insn
+| W  : insn
+| L  : id -> insn
+| S  : id -> insn
+| B  : bop -> insn
+| C  : nat -> insn
+| J  : nat -> insn
+| JT : nat -> insn
+| JF : nat -> insn.
+
+(* Program *)
+Definition prog := list insn.
+
+(* Subprogram *)
+Notation "p '<[' k ']>'" := (suffix insn p k) (at level 0, no associativity).
+
+Definition subprogram p k n := firstn n p<[k]>.
+
+Notation "p '<[' k ':' n ]>" := (subprogram p k n) (at level 39, no associativity).
+
+(* Configuration *)
+Definition conf := (list Z * state Z * list Z * list Z)%type.
+
+(* Big-step evaluation relation *)
+Reserved Notation "p '|-' c1 '--' q '-->' c2" (at level 0).
+Notation "st [ x '<-' y ]" := (update Z st x y) (at level 0).
+
+Inductive sm_int : prog -> conf -> prog -> conf -> Prop :=
+| sm_End   : forall (p : prog) (c : conf), p |- c -- [] --> c
+| sm_Read  : forall (p q : prog) (z : Z) (m : state Z) (s i o : list Z) (c' : conf), 
+               p |- (z::s, m, i, o) -- q --> c' -> p |- (s, m, z::i, o) -- R::q --> c'
+| sm_Write : forall (p q : prog) (z : Z) (m : state Z) (s i o : list Z) (c' : conf), 
+               p |- (s, m, i, z::o) -- q --> c' -> p |- (z::s, m, i, o) -- W::q --> c'
+| sm_Load  : forall (p q : prog) (x : id) (z : Z) (m : state Z) (s i o : list Z) (c' : conf), 
+               m / x => z -> p |- (z::s, m, i, o) -- q --> c' -> p |- (s, m, i, o) -- (L x)::q --> c'
+| sm_Store : forall (p q : prog) (x : id) (z : Z) (m : state Z) (s i o : list Z) (c' : conf), 
+               p |- (s, m [x <- z], i, o) -- q --> c' -> p |- (z::s, m, i, o) -- (S x)::q --> c'
+| sm_Add   : forall (p q : prog) (x y : Z) (m : state Z) (s i o : list Z) (c' : conf), 
+               p |- ((x + y)%Z::s, m, i, o) -- q --> c' -> p |- (y::x::s, m, i, o) -- (B Add)::q --> c'
+| sm_Sub   : forall (p q : prog) (x y : Z) (m : state Z) (s i o : list Z) (c' : conf), 
+               p |- ((x - y)%Z::s, m, i, o) -- q --> c' -> p |- (y::x::s, m, i, o) -- (B Sub)::q --> c'
+| sm_Mul   : forall (p q : prog) (x y : Z) (m : state Z) (s i o : list Z) (c' : conf), 
+               p |- ((x * y)%Z::s, m, i, o) -- q --> c' -> p |- (y::x::s, m, i, o) -- (B Mul)::q --> c'
+| sm_Div   : forall (p q : prog) (x y : Z) (m : state Z) (s i o : list Z) (c' : conf), 
+               p |- ((Z.div x y)::s, m, i, o) -- q --> c' -> p |- (y::x::s, m, i, o) -- (B Div)::q --> c'
+| sm_Mod   : forall (p q : prog) (x y : Z) (m : state Z) (s i o : list Z) (c' : conf), 
+               p |- ((Z.modulo x y)::s, m, i, o) -- q --> c' -> p |- (y::x::s, m, i, o) -- (B Mod)::q --> c'
+| sm_Le_T  : forall (p q : prog) (x y : Z) (m : state Z) (s i o : list Z) (c' : conf), 
+               Z.le x y -> p |- (Z.one::s, m, i, o) -- q --> c' -> p |- (y::x::s, m, i, o) -- (B Le)::q --> c'
+| sm_Le_F  : forall (p q : prog) (x y : Z) (m : state Z) (s i o : list Z) (c' : conf), 
+               Z.gt x y -> p |- (Z.zero::s, m, i, o) -- q --> c' -> p |- (y::x::s, m, i, o) -- (B Le)::q --> c'
+| sm_Ge_T  : forall (p q : prog) (x y : Z) (m : state Z) (s i o : list Z) (c' : conf), 
+               Z.ge x y -> p |- (Z.one::s, m, i, o) -- q --> c' -> p |- (y::x::s, m, i, o) -- (B Ge)::q --> c'
+| sm_Ge_F  : forall (p q : prog) (x y : Z) (m : state Z) (s i o : list Z) (c' : conf), 
+               Z.lt x y -> p |- (Z.zero::s, m, i, o) -- q --> c' -> p |- (y::x::s, m, i, o) -- (B Ge)::q --> c'
+| sm_Lt_T  : forall (p q : prog) (x y : Z) (m : state Z) (s i o : list Z) (c' : conf), 
+               Z.lt x y -> p |- (Z.one::s, m, i, o) -- q --> c' -> p |- (y::x::s, m, i, o) -- (B Lt)::q --> c'
+| sm_Lt_F  : forall (p q : prog) (x y : Z) (m : state Z) (s i o : list Z) (c' : conf), 
+               Z.ge x y -> p |- (Z.zero::s, m, i, o) -- q --> c' -> p |- (y::x::s, m, i, o) -- (B Lt)::q --> c'
+| sm_Gt_T  : forall (p q : prog) (x y : Z) (m : state Z) (s i o : list Z) (c' : conf), 
+               Z.gt x y -> p |- (Z.one::s, m, i, o) -- q --> c' -> p |- (y::x::s, m, i, o) -- (B Gt)::q --> c'
+| sm_Gt_F  : forall (p q : prog) (x y : Z) (m : state Z) (s i o : list Z) (c' : conf), 
+               Z.le x y -> p |- (Z.zero::s, m, i, o) -- q --> c' -> p |- (y::x::s, m, i, o) -- (B Gt)::q --> c'
+| sm_Eq_T  : forall (p q : prog) (x y : Z) (m : state Z) (s i o : list Z) (c' : conf), 
+               Z.eq x y -> p |- (Z.one::s, m, i, o) -- q --> c' -> p |- (y::x::s, m, i, o) -- (B Eq)::q --> c'
+| sm_Eq_F  : forall (p q : prog) (x y : Z) (m : state Z) (s i o : list Z) (c' : conf), 
+               ~ Z.eq x y -> p |- (Z.zero::s, m, i, o) -- q --> c' -> p |- (y::x::s, m, i, o) -- (B Eq)::q --> c'
+| sm_Ne_T  : forall (p q : prog) (x y : Z) (m : state Z) (s i o : list Z) (c' : conf), 
+               ~ Z.eq x y -> p |- (Z.one::s, m, i, o) -- q --> c' -> p |- (y::x::s, m, i, o) -- (B Ne)::q --> c'
+| sm_Ne_F  : forall (p q : prog) (x y : Z) (m : state Z) (s i o : list Z) (c' : conf), 
+               Z.eq x y -> p |- (Z.zero::s, m, i, o) -- q --> c' -> p |- (y::x::s, m, i, o) -- (B Ne)::q --> c'
+| sm_And   : forall (p q : prog) (x y : Z) (m : state Z) (s i o : list Z) (c' : conf), 
+               zbool x -> zbool y -> p |- ((x * y)%Z::s, m, i, o) -- q --> c' -> p |- (y::x::s, m, i, o) -- (B And)::q --> c'
+| sm_Or    : forall (p q : prog) (x y : Z) (m : state Z) (s i o : list Z) (c' : conf), 
+               zbool x -> zbool y -> p |- ((zor x y)::s, m, i, o) -- q --> c' -> p |- (y::x::s, m, i, o) -- (B Or)::q --> c'
+| sm_Const : forall (p q : prog) (n : nat) (m : state Z) (s i o : list Z) (c' : conf), 
+               p |- ((Z.of_nat n)::s, m, i, o) -- q --> c' -> p |- (s, m, i, o) -- (C n)::q --> c'
+| sm_J     : forall (p q : prog) (n : nat) (c c' : conf), 
+               p |- c -- p<[n]> --> c' -> p |- c -- (J n)::q --> c'
+| sm_JT_T  : forall (p q : prog) (n : nat) (m : state Z) (s i o : list Z) (c' : conf), 
+               p |- (s, m, i, o) -- p<[n]> --> c' -> p |- (Z.one::s, m, i, o) -- (JT n)::q --> c'
+| sm_JT_F  : forall (p q : prog) (n : nat) (m : state Z) (s i o : list Z) (c' : conf), 
+               p |- (s, m, i, o) -- q --> c' -> p |- (Z.zero::s, m, i, o) -- (JT n)::q --> c'
+| sm_JF_T  : forall (p q : prog) (n : nat) (m : state Z) (s i o : list Z) (c' : conf), 
+               p |- (s, m, i, o) -- q --> c' -> p |- (Z.one::s, m, i, o) -- (JT n)::q --> c'
+| sm_JF_F  : forall (p q : prog) (n : nat) (m : state Z) (s i o : list Z) (c' : conf), 
+               p |- (s, m, i, o) -- p<[n]> --> c' -> p |- (Z.zero::s, m, i, o) -- (JT n)::q --> c'
+where "p '|-' c1 '--' q '-->' c2" := (sm_int p c1 q c2).
+
+(* Expression compiler *)
+Fixpoint compile_expr (e : expr) :=
+  match e with
+  | Var  x       => [L x]
+  | Nat  n       => [C n]
+  | Bop op e1 e2 => compile_expr e1 ++ compile_expr e2 ++ [B op]
+  end.
+
+(* Partial correctness of expression compiler *)
+Lemma compiled_expr_correct: forall (e : expr) (st : state Z) (s i o : list Z) (n : Z),
+                               [| e |] st => n -> (compile_expr e) |- (s, st, i, o) -- (compile_expr e) --> (n::s, st, i, o).
+Proof. admit. Admitted.
